mutable_typed_shared_data: seal_pred as a whole invariant

theories/examples/mutable_typed_shared_data/invariants.v
@@ -7,27 +7,24 @@ Section invariants.
   Context {Σ:gFunctors} {memg:memG Σ} {regg:regG Σ} {sealsg: sealStoreG Σ}
           {nainv: logrel_na_invs Σ} `{MP: MachineParameters}.
 
-  (*  *)
-  (* Note: *)
-  Definition seal_pred τ Φ {Hpers : ∀ w, Persistent (Φ w)} := seal_pred τ Φ.
+  (* `seal_pred` denotes that the sealed satisfies a predicate `Φ`, for a specific `τ` OType. *)
+  (* Note: `seal_pred` does not need to be put inside an invariant, because it is `Persistent`. *)
+  Definition seal_pred τ Φ {Hpers : ∀ w, Persistent (Φ w)} := seal_store.seal_pred τ Φ.
 
-  (* `seal_state` is the combination of `seal_pred` and a specific invariant. *)
-  (* This invariant pin `WSealRange` in memory to retrieve an access to it. *)
-  (* > In our case, `WSealRange` is already pinned and easily accessible. *)
-  (* For simplicity, this example will only use `seal_pred`. *)
+  (* Note: `arch_sealing.seal_state` is the combination of `seal_pred` and a invariant. *)
+  (* > This invariant pins `WSealRange` in memory to retrieve an access to it. *)
+  (* For simplicity, we will explicitly split `seal_pred` and the invariant on `WSealRange`. *)
 
-  (* Fact that the value `w` has been validly sealed satisfying a `Φ` predicate. *)
-  (* This definition is close to `interp_sb` and can be obtained using `interp_valid_sealed`. *)
-  Definition valid_sealed w τ Φ := valid_sealed w τ Φ.
+  (* Fact that the value `w`, if `interp w`, has been validly sealed satisfying a `Φ` predicate. *)
+  Definition valid_sealed w τ Φ := arch_sealing.valid_sealed w τ Φ.
 
-  (* Something sealed is enough to know that the sealed satisfies a predicate `Φ`. *)
-  (* The predicate `Φ` can be refined to a concrete predicate with `seal_pred_valid_sealed_eq`. *)
-  Definition interp_valid_sealed sb τ := interp_valid_sealed sb τ.
+  (* Lemma: If something is sealed, it is sufficient to know that the sealed satisfies a predicate `Φ`. *)
+  Definition interp_valid_sealed sb τ := arch_sealing.interp_valid_sealed sb τ.
 
-  (* Concludes that `Φ` ≡ `Φ'` if `seal_state` and `valid_sealed` have the same `τ` OType. *)
-  (* Note: This is a more-generic version of `sealLL_valid_sealed_pred_eq` *)
+  (* Lemma: Concludes that `Φ ≡ Φ'` if `seal_pred τ Φ` and `valid_sealed w τ Φ` have the same `τ` OType. *)
+  (* Note: This is a more generic version of `arch_sealing.sealLL_valid_sealed_pred_eq` *)
   Lemma seal_pred_valid_sealed_eq τ w Φ Φ' {Hpers : ∀ w, Persistent (Φ w)} :
-    seal_store.seal_pred τ Φ -∗ valid_sealed w τ Φ' -∗ (∀ w, ▷ (Φ w ≡ Φ' w)).
+    seal_pred τ Φ -∗ valid_sealed w τ Φ' -∗ (∀ w, ▷ (Φ w ≡ Φ' w)).
   Proof.
     iIntros "Hsp Hvs".
     iDestruct "Hvs" as (sb) "(_ & _ & Hsp' & _)".
@@ -36,29 +33,37 @@ Section invariants.
 
 End invariants.
 
+(* The proof guideline for accessing the sealed predicate is as follows: *)
+
+(* We assume: *)
+(*  - `seal_pred τ φ`, for some known `φ` (e.g: `sealed_int`) *)
+(*  - `interp w`, where `w = WSealed τ scap` for any given `scap` *)
+
+(* 1. Using `interp_valid_sealed`, we can get `▷ valid_sealed (WSealed τ scap) τ Φ`. *)
+(* 2. `Φ` is currently unknown, we have to use `seal_pred_valid_sealed_eq` to retrieve `φ`. *)
+
 Section invariants_int.
   Context {Σ:gFunctors} {memg:memG Σ} {regg:regG Σ} {sealsg: sealStoreG Σ}
           {nainv: logrel_na_invs Σ} `{MP: MachineParameters}.
 
   Definition seal_intN : namespace := nroot .@ "seal".
 
-  Definition int_sealed : Word → iProp Σ :=
-    (λ w, (∃ a_cap, ⌜w = WCap RW a_cap (a_cap ^+ 1)%a a_cap⌝
-                         ∗ na_inv logrel_nais seal_intN (∃ w, a_cap ↦ₐ w ∗ ⌜is_z w⌝))%I).
+  (* `sealed_int` is the sealed predicate of a sealed buffer containing an integer. *)
+  Definition sealed_int : Word → iProp Σ :=
+    λ w, na_inv logrel_nais seal_intN
+           (∃ a_cap, ⌜w = WCap RW a_cap (a_cap ^+ 1)%a a_cap⌝ ∗ (∃ w, a_cap ↦ₐ w ∗ ⌜is_z w⌝))%I.
 
-  Instance int_sealed_persistent w : Persistent (int_sealed w).
+  (* Note: `sealed_int` is not `Timeless` because of the use of the non-atomic invariant. *)
+  (* > In our case, any later can be stripped at time. *)
+  (* One could use `a_cap ↦ₐ{DFracDiscarded} w` to avoid using the non-atomic invariant. *)
+  (* > However, this denies the right to write to `a_cap` making it read-only. *)
+
+  (* Required by `seal_pred`: `sealed_int` is `Persistent`. *)
+  Instance sealed_int_persistent w : Persistent (sealed_int w).
   Proof. apply _. Qed.
 
   (* Integer-specific redefinitions *)
-  Definition seal_pred_int τ := seal_pred τ int_sealed.
-  Definition valid_sealed_int w τ := valid_sealed w τ int_sealed.
-
-  Lemma seal_state_int_valid_sealed_pred_eq τ w Φ :
-    seal_pred τ int_sealed -∗ valid_sealed w τ Φ -∗  (∀ w, ▷ (int_sealed w ≡ Φ w)).
-  Proof.
-    iIntros "Hsp Hvs".
-    iDestruct "Hvs" as (sb) "(_ & _ & Hsp' & _)".
-    iApply (seal_pred_agree with "Hsp Hsp'").
-  Qed.
+  Definition seal_pred_int τ := seal_pred τ sealed_int.
+  Definition valid_sealed_int w τ := valid_sealed w τ sealed_int.
 
 End invariants_int.
